p256: rm extra functions in Hacl.Spec.P256.Math

code/ecdsap256/Hacl.Impl.P256.Field.fst
@@ -1,38 +1,32 @@
 module Hacl.Impl.P256.Field
 
+open FStar.Mul
 open FStar.HyperStack.All
 open FStar.HyperStack
 module ST = FStar.HyperStack.ST
-
-open FStar.Mul
-open FStar.Math.Lemmas
 
 open Lib.IntTypes
 open Lib.Buffer
 open Lib.IntTypes.Intrinsics
 
-open Spec.P256
-open Hacl.Spec.P256.Lemmas
-open Hacl.Spec.P256.MontgomeryMultiplication
-
+open Hacl.Spec.P256.Math
 open Hacl.Spec.P256.Felem
 open Hacl.Impl.P256.Bignum
-open Hacl.Spec.P256.Math
 open Hacl.Impl.P256.Constants
+
+module S = Spec.P256
+module SM = Hacl.Spec.P256.MontgomeryMultiplication
+module SL = Hacl.Spec.P256.Lemmas
 
 #set-options "--z3rlimit 50 --fuel 0 --ifuel 0"
 
 inline_for_extraction noextract
-val reduction_prime_2prime_with_carry_impl:
-    cin:uint64
-  -> x:felem
-  -> result:felem ->
-  Stack unit
+val reduction_prime_2prime_with_carry_impl: cin:uint64 -> x:felem -> result:felem -> Stack unit
   (requires fun h ->
     live h x /\ live h result /\ eq_or_disjoint x result /\
-    (as_nat h x + uint_v cin * pow2 256) < 2 * prime)
+    (as_nat h x + uint_v cin * pow2 256) < 2 * S.prime)
   (ensures fun h0 _ h1 -> modifies (loc result) h0 h1 /\
-    as_nat h1 result = (as_nat h0 x + uint_v cin * pow2 256) % prime)
+    as_nat h1 result = (as_nat h0 x + uint_v cin * pow2 256) % S.prime)
 
 let reduction_prime_2prime_with_carry_impl cin x result =
   push_frame();
@@ -42,24 +36,24 @@ let reduction_prime_2prime_with_carry_impl cin x result =
     let c = bn_sub4_il x prime_buffer tempBuffer in
   let h0 = ST.get() in
       assert(uint_v c <= 1);
-      assert(if uint_v c = 0 then as_nat h0 x >= prime else as_nat h0 x < prime);
+      assert(if uint_v c = 0 then as_nat h0 x >= S.prime else as_nat h0 x < S.prime);
     let carry = sub_borrow_u64 c cin (u64 0) tempBufferForSubborrow in
     bn_cmovznz4 carry tempBuffer x result;
   let h1 = ST.get() in
       assert_norm (pow2 64 * pow2 64 * pow2 64 * pow2 64 = pow2 256);
-      assert_norm (prime < pow2 256);
-      assert_norm(pow2 256 < 2 * prime);
+      assert_norm (S.prime < pow2 256);
+      assert_norm(pow2 256 < 2 * S.prime);
 
       assert(uint_v cin <= 1);
       assert(uint_v c <= 1);
 
-      assert(if as_nat h0 x >= prime then uint_v c = 0 else True);
+      assert(if as_nat h0 x >= S.prime then uint_v c = 0 else True);
       assert(if uint_v cin < uint_v c then as_nat h1 result == as_nat h0 x else as_nat h1 result == as_nat h0 tempBuffer);
 
-      assert(as_nat h1 result < prime);
+      assert(as_nat h1 result < S.prime);
 
-      modulo_addition_lemma (as_nat h1 result) prime 1;
-      small_modulo_lemma_1 (as_nat h1 result) prime;
+      Math.Lemmas.modulo_addition_lemma (as_nat h1 result) S.prime 1;
+      Math.Lemmas.small_modulo_lemma_1 (as_nat h1 result) S.prime;
   pop_frame()
 
 
@@ -67,15 +61,15 @@ inline_for_extraction noextract
 val reduction_prime_2prime_8_with_carry_impl: x:widefelem -> res:felem -> Stack unit
   (requires fun h ->
     live h x /\ live h res /\ eq_or_disjoint x res /\
-    wide_as_nat h x < 2 * prime)
+    wide_as_nat h x < 2 * S.prime)
   (ensures fun h0 _ h1 -> modifies (loc res) h0 h1 /\
-    as_nat h1 res == wide_as_nat h0 x % prime)
+    as_nat h1 res == wide_as_nat h0 x % S.prime)
 
 let reduction_prime_2prime_8_with_carry_impl x result =
   push_frame();
     assert_norm (pow2 64 * pow2 64 * pow2 64 * pow2 64 = pow2 256);
-    assert_norm (prime < pow2 256);
-    assert_norm(pow2 256 < 2 * prime);
+    assert_norm (S.prime < pow2 256);
+    assert_norm(pow2 256 < 2 * S.prime);
     let h0 = ST.get() in
     let tempBuffer = create (size 4) (u64 0) in
     let tempBufferForSubborrow = create (size 1) (u64 0) in
@@ -86,36 +80,36 @@ let reduction_prime_2prime_8_with_carry_impl x result =
     let carry = sub_borrow_u64 c cin (u64 0) tempBufferForSubborrow in
     bn_cmovznz4 carry tempBuffer x_ result;
       let h4 = ST.get() in
-      assert_norm (pow2 256 > prime);
-      assert(if (wide_as_nat h0 x < prime) then begin
-      small_modulo_lemma_1 (wide_as_nat h0 x) prime;
-      as_nat h4 result = (wide_as_nat h0 x) % prime end
+      assert_norm (pow2 256 > S.prime);
+      assert(if (wide_as_nat h0 x < S.prime) then begin
+      Math.Lemmas.small_modulo_lemma_1 (wide_as_nat h0 x) S.prime;
+      as_nat h4 result = (wide_as_nat h0 x) % S.prime end
       else
 	begin
-	small_modulo_lemma_1 (as_nat h4 result) prime;
-	lemma_mod_sub (wide_as_nat h0 x) prime 1;
-	as_nat h4 result = (wide_as_nat h0 x) % prime
+	Math.Lemmas.small_modulo_lemma_1 (as_nat h4 result) S.prime;
+	Math.Lemmas.lemma_mod_sub (wide_as_nat h0 x) S.prime 1;
+	as_nat h4 result = (wide_as_nat h0 x) % S.prime
 	end );
  pop_frame()
 
 
-val lemma_reduction1_0: a:nat{a < pow2 256 /\ a >= prime} -> r:nat{r = a - prime} ->
-  Lemma (r = a % prime)
+val lemma_reduction1_0: a:nat{a < pow2 256 /\ a >= S.prime} -> r:nat{r = a - S.prime} ->
+  Lemma (r = a % S.prime)
 
 let lemma_reduction1_0 a r =
-  assert_norm (pow2 256 - prime < prime);
-  small_modulo_lemma_1 r prime;
-  lemma_mod_sub_distr a prime prime
+  assert_norm (pow2 256 - S.prime < S.prime);
+  Math.Lemmas.small_modulo_lemma_1 r S.prime;
+  Math.Lemmas.lemma_mod_sub_distr a S.prime S.prime
 
 
-val lemma_reduction1: a:nat{a < pow2 256} -> r:nat{if a >= prime then r = a - prime else r = a} ->
-  Lemma (r = a % prime)
+val lemma_reduction1: a:nat{a < pow2 256} -> r:nat{if a >= S.prime then r = a - S.prime else r = a} ->
+  Lemma (r = a % S.prime)
 
 let lemma_reduction1 a r =
-  if a >= prime then
+  if a >= S.prime then
    lemma_reduction1_0 a r
   else
-    small_mod r prime
+   Math.Lemmas.small_mod r S.prime
 
 
 [@CInline]
@@ -140,7 +134,7 @@ val lemma_t_computation: t: uint64{uint_v t == 0 \/ uint_v t == 1} ->
 	let t2 = (u64 0) -. t in
 	let t3 = (t <<. (size 32)) -. (t <<. (size 1)) in
 	let s = uint_v t0 + uint_v t1 * pow2 64 + uint_v t2 * pow2 128 + uint_v t3 * pow2 192 in
-	if uint_v t = 1 then s == pow2 256 - prime - 1 else s == 0
+	if uint_v t = 1 then s == pow2 256 - S.prime - 1 else s == 0
     )
 
 let lemma_t_computation t =
@@ -149,7 +143,7 @@ let lemma_t_computation t =
   let t2 = (u64 0) -. t in
   let t3 = (t <<. (size 32)) -. (t <<. (size 1)) in
   let s = uint_v t0 + uint_v t1 * pow2 64 + uint_v t2 * pow2 128 + uint_v t3 * pow2 192 in
-  assert_norm(18446744069414584320 * pow2 64 + 18446744073709551615 * pow2 128 + 4294967294 * pow2 192 = pow2 256 - prime - 1)
+  assert_norm(18446744069414584320 * pow2 64 + 18446744073709551615 * pow2 128 + 4294967294 * pow2 192 = pow2 256 - S.prime - 1)
 
 
 val lemma_t_computation2: t: uint64 {uint_v t == 0 \/ uint_v t == 1} ->
@@ -160,7 +154,7 @@ val lemma_t_computation2: t: uint64 {uint_v t == 0 \/ uint_v t == 1} ->
       let t2 = u64 0 in
       let t3 = t -. (t <<. (size 32)) in
       let s = uint_v t0 + uint_v t1 * pow2 64 + uint_v t2 * pow2 128 + uint_v t3 * pow2 192 in
-      if uint_v t = 1 then s == prime else s == 0
+      if uint_v t = 1 then s == S.prime else s == 0
     )
 
 let lemma_t_computation2 t =
@@ -169,7 +163,7 @@ let lemma_t_computation2 t =
   let t2 = u64 0 in
   let t3 = t -. (t <<. (size 32)) in
   let s = uint_v t0 + uint_v t1 * pow2 64 + uint_v t2 * pow2 128 + uint_v t3 * pow2 192 in
-  assert_norm(18446744073709551615 + 4294967295 * pow2 64 + 18446744069414584321 * pow2 192 = prime)
+  assert_norm(18446744073709551615 + 4294967295 * pow2 64 + 18446744069414584321 * pow2 192 = S.prime)
 
 
 [@CInline]
@@ -179,8 +173,8 @@ let fadd x y out =
   lemma_t_computation t;
   reduction_prime_2prime_with_carry_impl t out out;
   let h2 = ST.get() in
-  additionInDomain (as_nat h0 x) (as_nat h0 y);
-  inDomain_mod_is_not_mod (fromDomain_ (as_nat h0 x) + fromDomain_ (as_nat h0 y))
+  SM.additionInDomain (as_nat h0 x) (as_nat h0 y);
+  SM.inDomain_mod_is_not_mod (SM.fromDomain_ (as_nat h0 x) + SM.fromDomain_ (as_nat h0 y))
 
 
 let fdouble x out =
@@ -198,22 +192,22 @@ let fsub x y out =
   let t1 = ((u64 0) -. t) >>. (size 32) in
   let t2 = u64 0 in
   let t3 = t -. (t <<. (size 32)) in
-    modulo_addition_lemma  (as_nat h0 x - as_nat h0 y) prime 1;
+    Math.Lemmas.modulo_addition_lemma  (as_nat h0 x - as_nat h0 y) S.prime 1;
   let c = bn_add4_variables out (u64 0)  t0 t1 t2 t3 out in
     let h2 = ST.get() in
       assert(
       if as_nat h0 x - as_nat h0 y >= 0 then
 	begin
-	  modulo_lemma (as_nat h0 x - as_nat h0 y) prime;
-	  as_nat h2 out == (as_nat h0 x - as_nat h0 y) % prime
+	  Math.Lemmas.modulo_lemma (as_nat h0 x - as_nat h0 y) S.prime;
+	  as_nat h2 out == (as_nat h0 x - as_nat h0 y) % S.prime
 	end
       else
           begin
-	    modulo_lemma (as_nat h2 out) prime;
-            as_nat h2 out == (as_nat h0 x - as_nat h0 y) % prime
+	    Math.Lemmas.modulo_lemma (as_nat h2 out) S.prime;
+            as_nat h2 out == (as_nat h0 x - as_nat h0 y) % S.prime
 	  end);
-    substractionInDomain (felem_seq_as_nat (as_seq h0 x)) (felem_seq_as_nat (as_seq h0 y));
-    inDomain_mod_is_not_mod (fromDomain_ (felem_seq_as_nat (as_seq h0 x)) - fromDomain_ (felem_seq_as_nat (as_seq h0 y)))
+    SM.substractionInDomain (felem_seq_as_nat (as_seq h0 x)) (felem_seq_as_nat (as_seq h0 y));
+    SM.inDomain_mod_is_not_mod (SM.fromDomain_ (felem_seq_as_nat (as_seq h0 x)) - SM.fromDomain_ (felem_seq_as_nat (as_seq h0 y)))
 
 //--------------------------------------
 
@@ -222,22 +216,22 @@ val add8_without_carry1: t:widefelem -> t1:widefelem -> result:widefelem -> Stac
   (requires fun h ->
     live h t /\ live h t1 /\ live h result /\
     eq_or_disjoint t1 t /\ eq_or_disjoint t1 result /\ eq_or_disjoint t result /\
-    wide_as_nat h t1 < pow2 320 /\ wide_as_nat h t < prime * prime)
+    wide_as_nat h t1 < pow2 320 /\ wide_as_nat h t < S.prime * S.prime)
   (ensures fun h0 _ h1 -> modifies (loc result) h0 h1 /\
     wide_as_nat h1 result = wide_as_nat h0 t + wide_as_nat h0 t1)
 
 let add8_without_carry1 t t1 result  =
   let _  = bn_add8 t t1 result in
-    assert_norm (pow2 320 + prime * prime < pow2 512)
+    assert_norm (pow2 320 + S.prime * S.prime < pow2 512)
 
 
 inline_for_extraction noextract
 val montgomery_multiplication_round: t:widefelem -> round:widefelem -> Stack unit
   (requires fun h ->
     live h t /\ live h round /\
-    wide_as_nat h t < prime * prime)
+    wide_as_nat h t < S.prime * S.prime)
   (ensures fun h0 _ h1 -> modifies (loc round) h0 h1 /\
-    wide_as_nat h1 round = (wide_as_nat h0 t + prime * (wide_as_nat h0 t % pow2 64)) / pow2 64)
+    wide_as_nat h1 round = (wide_as_nat h0 t + S.prime * (wide_as_nat h0 t % pow2 64)) / pow2 64)
 
 let montgomery_multiplication_round t round =
   push_frame();
@@ -253,53 +247,53 @@ let montgomery_multiplication_round t round =
 
 
 val montgomery_multiplication_one_round_proof:
-  t: nat {t < prime * prime} ->
-  result: nat {result = (t + (t % pow2 64) * prime) / pow2 64} ->
-  co: nat {co % prime == t % prime} -> Lemma (
-    result % prime == co * modp_inv2 (pow2 64) % prime /\
-    result < prime * prime)
+  t: nat {t < S.prime * S.prime} ->
+  result: nat {result = (t + (t % pow2 64) * S.prime) / pow2 64} ->
+  co: nat {co % S.prime == t % S.prime} -> Lemma (
+    result % S.prime == co * S.modp_inv2 (pow2 64) % S.prime /\
+    result < S.prime * S.prime)
 
 let montgomery_multiplication_one_round_proof t result co =
-  mult_one_round t co;
-  mul_lemma_1 (t % pow2 64) (pow2 64) prime;
-  assert_norm (prime * prime + pow2 64 * prime < pow2 575);
-  lemma_div_lt (t + (t % pow2 64) * prime) 575 64;
-  assert_norm (prime * prime > pow2 (575 - 64))
+  SL.mult_one_round t co;
+  SL.mul_lemma_1 (t % pow2 64) (pow2 64) S.prime;
+  assert_norm (S.prime * S.prime + pow2 64 * S.prime < pow2 575);
+  Math.Lemmas.lemma_div_lt (t + (t % pow2 64) * S.prime) 575 64;
+  assert_norm (S.prime * S.prime > pow2 (575 - 64))
 
 
 inline_for_extraction noextract
 val montgomery_multiplication_round_twice: t: widefelem -> result: widefelem -> Stack unit
-  (requires fun h -> live h t /\ live h result  /\ wide_as_nat h t < prime * prime)
+  (requires fun h -> live h t /\ live h result  /\ wide_as_nat h t < S.prime * S.prime)
   (ensures fun h0 _ h1 ->
     modifies (loc result) h0 h1 /\
     (
-      let round = (wide_as_nat h0 t + prime * (wide_as_nat h0 t % pow2 64)) / pow2 64 in
-      wide_as_nat h1 result < prime * prime /\
-      wide_as_nat h1 result % prime == (wide_as_nat h0 t * modp_inv2_prime (pow2 128) prime) % prime /\
-      wide_as_nat h1 result == (round + prime * (round % pow2 64)) / pow2 64
+      let round = (wide_as_nat h0 t + S.prime * (wide_as_nat h0 t % pow2 64)) / pow2 64 in
+      wide_as_nat h1 result < S.prime * S.prime /\
+      wide_as_nat h1 result % S.prime == (wide_as_nat h0 t * S.modp_inv2_prime (pow2 128) S.prime) % S.prime /\
+      wide_as_nat h1 result == (round + S.prime * (round % pow2 64)) / pow2 64
     )
  )
 
 let montgomery_multiplication_round_twice t result =
-  assert_norm(prime > 3);
+  assert_norm(S.prime > 3);
   push_frame();
     let tempRound = create (size 8) (u64 0) in
       let h0 = ST.get() in
     montgomery_multiplication_round t tempRound;
       let h1 = ST.get() in
-      Math.Lemmas.swap_mul (wide_as_nat h0 t % pow2 64) prime;
+      Math.Lemmas.swap_mul (wide_as_nat h0 t % pow2 64) S.prime;
       montgomery_multiplication_one_round_proof (wide_as_nat h0 t) (wide_as_nat h1 tempRound) (wide_as_nat h0 t);
     montgomery_multiplication_round tempRound result;
       let h2 = ST.get() in
-      Math.Lemmas.swap_mul (wide_as_nat h1 tempRound % pow2 64) prime;
-      montgomery_multiplication_one_round_proof (wide_as_nat h1 tempRound) (wide_as_nat h2 result) (wide_as_nat h0 t * modp_inv2_prime (pow2 64) prime);
+      Math.Lemmas.swap_mul (wide_as_nat h1 tempRound % pow2 64) S.prime;
+      montgomery_multiplication_one_round_proof (wide_as_nat h1 tempRound) (wide_as_nat h2 result) (wide_as_nat h0 t * S.modp_inv2_prime (pow2 64) S.prime);
       lemma_montgomery_mod_inverse_addition (wide_as_nat h0 t);
   pop_frame()
 
 
 [@CInline]
 let montgomery_multiplication_buffer_by_one a result =
-  assert_norm (prime > 3);
+  assert_norm (S.prime > 3);
   push_frame();
     let t = create (size 8) (u64 0) in
       let t_low = sub t (size 0) (size 4) in
@@ -310,32 +304,32 @@ let montgomery_multiplication_buffer_by_one a result =
     copy t_low a;
       let h1 = ST.get() in
       assert(wide_as_nat h0 t = as_nat h0 t_low + as_nat h0 t_high * pow2 256);
-      assert_norm (prime < prime * prime);
+      assert_norm (S.prime < S.prime * S.prime);
     montgomery_multiplication_round_twice t round2;
       let h2 = ST.get() in
     montgomery_multiplication_round_twice round2 round4;
       lemma_montgomery_mod_inverse_addition2 (wide_as_nat h1 t);
-      lemma_mod_mul_distr_l (wide_as_nat h2 round2) (modp_inv2_prime (pow2 128) prime) prime;
-      lemma_mod_mul_distr_l (wide_as_nat h1 t * modp_inv2_prime (pow2 128) prime) (modp_inv2_prime (pow2 128) prime) prime;
-	mul_lemma_2 (wide_as_nat h1 t % pow2 64) (pow2 64 - 1) prime;
-	mul_lemma_2 (let round = (wide_as_nat h1 t + prime * (wide_as_nat h1 t % pow2 64)) / pow2 64 in round % pow2 64) (pow2 64 - 1) prime;
-	mul_lemma_2 (
-	  let round = (wide_as_nat h1 t + prime * (wide_as_nat h1 t % pow2 64)) / pow2 64 in
-	  let round2 = (round + prime * (round % pow2 64)) / pow2 64 in
-	  round2 % pow2 64) (pow2 64 - 1) prime;
-	mul_lemma_2 (
-	  let round = (wide_as_nat h1 t + prime * (wide_as_nat h1 t % pow2 64)) / pow2 64 in
-	  let round2 = (round + prime * (round % pow2 64)) / pow2 64 in
-	  let round3 = (round2 + prime * (round2 % pow2 64)) / pow2 64 in
-	  round3 % pow2 64) (pow2 64 - 1) prime;
+      Math.Lemmas.lemma_mod_mul_distr_l (wide_as_nat h2 round2) (S.modp_inv2_prime (pow2 128) S.prime) S.prime;
+      Math.Lemmas.lemma_mod_mul_distr_l (wide_as_nat h1 t * S.modp_inv2_prime (pow2 128) S.prime) (S.modp_inv2_prime (pow2 128) S.prime) S.prime;
+	SL.mul_lemma_2 (wide_as_nat h1 t % pow2 64) (pow2 64 - 1) S.prime;
+	SL.mul_lemma_2 (let round = (wide_as_nat h1 t + S.prime * (wide_as_nat h1 t % pow2 64)) / pow2 64 in round % pow2 64) (pow2 64 - 1) S.prime;
+	SL.mul_lemma_2 (
+	  let round = (wide_as_nat h1 t + S.prime * (wide_as_nat h1 t % pow2 64)) / pow2 64 in
+	  let round2 = (round + S.prime * (round % pow2 64)) / pow2 64 in
+	  round2 % pow2 64) (pow2 64 - 1) S.prime;
+	SL.mul_lemma_2 (
+	  let round = (wide_as_nat h1 t + S.prime * (wide_as_nat h1 t % pow2 64)) / pow2 64 in
+	  let round2 = (round + S.prime * (round % pow2 64)) / pow2 64 in
+	  let round3 = (round2 + S.prime * (round2 % pow2 64)) / pow2 64 in
+	  round3 % pow2 64) (pow2 64 - 1) S.prime;
     reduction_prime_2prime_8_with_carry_impl round4 result;
-    lemmaFromDomain (as_nat h0 a);
+    SM.lemmaFromDomain (as_nat h0 a);
   pop_frame()
 
 
 [@CInline]
 let fmul a b result =
-  assert_norm(prime > 3);
+  assert_norm(S.prime > 3);
   push_frame();
     let t = create (size 8) (u64 0) in
     let round2 = create (size 8) (u64 0) in
@@ -343,40 +337,40 @@ let fmul a b result =
       let h0 = ST.get() in
     bn_mul4 a b t;
       let h1 = ST.get() in
-      mul_lemma_ (as_nat h0 a) (as_nat h0 b) prime;
+      SL.mul_lemma_ (as_nat h0 a) (as_nat h0 b) S.prime;
   montgomery_multiplication_round_twice t round2;
       let h2 = ST.get() in
   montgomery_multiplication_round_twice round2 round4;
       let h3 = ST.get() in
 	lemma_montgomery_mod_inverse_addition2 (wide_as_nat h1 t);
-	lemma_mod_mul_distr_l (wide_as_nat h2 round2) (modp_inv2_prime (pow2 128) prime) prime;
-	lemma_mod_mul_distr_l (wide_as_nat h1 t * modp_inv2_prime (pow2 128) prime) (modp_inv2_prime (pow2 128) prime) prime;
-      mul_lemma_2 (wide_as_nat h1 t % pow2 64) (pow2 64 - 1) prime;
-      mul_lemma_ (as_nat h0 a) (as_nat h0 b) prime;
-      mul_lemma_1 (
-         let round = (wide_as_nat h1 t + prime * (wide_as_nat h1 t % pow2 64)) / pow2 64 in
-	 round % pow2 64) (pow2 64) prime;
-      mul_lemma_1 (
-	let round = (wide_as_nat h1 t + prime * (wide_as_nat h1 t % pow2 64)) / pow2 64 in
-	let round2 = (round + prime * (round % pow2 64)) / pow2 64 in
-	round2 % pow2 64) (pow2 64) prime;
-      mul_lemma_1 (
-	let round = (wide_as_nat h1 t + prime * (wide_as_nat h1 t % pow2 64)) / pow2 64 in
-	let round2 = (round + prime * (round % pow2 64)) / pow2 64 in
-	let round3 = (round2 + prime * (round2 % pow2 64)) / pow2 64 in
-	round3 % pow2 64) (pow2 64) prime;
-      assert_norm((prime * pow2 64 + (prime * pow2 64 + (prime * pow2 64 + ((pow2 64 - 1) * prime + prime * prime) / pow2 64) / pow2 64)/ pow2 64) / pow2 64 < 2 * prime);
+	Math.Lemmas.lemma_mod_mul_distr_l (wide_as_nat h2 round2) (S.modp_inv2_prime (pow2 128) S.prime) S.prime;
+	Math.Lemmas.lemma_mod_mul_distr_l (wide_as_nat h1 t * S.modp_inv2_prime (pow2 128) S.prime) (S.modp_inv2_prime (pow2 128) S.prime) S.prime;
+      SL.mul_lemma_2 (wide_as_nat h1 t % pow2 64) (pow2 64 - 1) S.prime;
+      SL.mul_lemma_ (as_nat h0 a) (as_nat h0 b) S.prime;
+      SL.mul_lemma_1 (
+         let round = (wide_as_nat h1 t + S.prime * (wide_as_nat h1 t % pow2 64)) / pow2 64 in
+	 round % pow2 64) (pow2 64) S.prime;
+      SL.mul_lemma_1 (
+	let round = (wide_as_nat h1 t + S.prime * (wide_as_nat h1 t % pow2 64)) / pow2 64 in
+	let round2 = (round + S.prime * (round % pow2 64)) / pow2 64 in
+	round2 % pow2 64) (pow2 64) S.prime;
+      SL.mul_lemma_1 (
+	let round = (wide_as_nat h1 t + S.prime * (wide_as_nat h1 t % pow2 64)) / pow2 64 in
+	let round2 = (round + S.prime * (round % pow2 64)) / pow2 64 in
+	let round3 = (round2 + S.prime * (round2 % pow2 64)) / pow2 64 in
+	round3 % pow2 64) (pow2 64) S.prime;
+      assert_norm((S.prime * pow2 64 + (S.prime * pow2 64 + (S.prime * pow2 64 + ((pow2 64 - 1) * S.prime + S.prime * S.prime) / pow2 64) / pow2 64)/ pow2 64) / pow2 64 < 2 * S.prime);
   reduction_prime_2prime_8_with_carry_impl round4 result;
-  lemmaFromDomainToDomain (as_nat h0 a);
-  lemmaFromDomainToDomain (as_nat h0 b);
-  multiplicationInDomainNat #(fromDomain_ (as_nat h0 a)) #(fromDomain_ (as_nat h0 b))  (as_nat h0 a) (as_nat h0 b);
-  inDomain_mod_is_not_mod (fromDomain_ (as_nat h0 a) * fromDomain_ (as_nat h0 b));
+  SM.lemmaFromDomainToDomain (as_nat h0 a);
+  SM.lemmaFromDomainToDomain (as_nat h0 b);
+  SM.multiplicationInDomainNat #(SM.fromDomain_ (as_nat h0 a)) #(SM.fromDomain_ (as_nat h0 b))  (as_nat h0 a) (as_nat h0 b);
+  SM.inDomain_mod_is_not_mod (SM.fromDomain_ (as_nat h0 a) * SM.fromDomain_ (as_nat h0 b));
   pop_frame()
 
 
 [@CInline]
 let fsqr a result =
-  assert_norm(prime > 3);
+  assert_norm(S.prime > 3);
   push_frame();
     let t = create (size 8) (u64 0) in
     let round2 = create (size 8) (u64 0) in
@@ -384,33 +378,33 @@ let fsqr a result =
       let h0 = ST.get() in
     bn_sqr4 a t;
       let h1 = ST.get() in
-      mul_lemma_ (as_nat h0 a) (as_nat h0 a) prime;
+      SL.mul_lemma_ (as_nat h0 a) (as_nat h0 a) S.prime;
   montgomery_multiplication_round_twice t round2;
       let h2 = ST.get() in
   montgomery_multiplication_round_twice round2 round4;
       let h3 = ST.get() in
   lemma_montgomery_mod_inverse_addition2 (wide_as_nat h1 t);
-  lemma_mod_mul_distr_l (wide_as_nat h2 round2) (modp_inv2_prime (pow2 128) prime) prime;
-  lemma_mod_mul_distr_l (wide_as_nat h1 t * modp_inv2_prime (pow2 128) prime) (modp_inv2_prime (pow2 128) prime) prime;
-      mul_lemma_2 (wide_as_nat h1 t % pow2 64) (pow2 64 - 1) prime;
-      mul_lemma_ (as_nat h0 a) (as_nat h0 a) prime;
-      mul_lemma_1 (
-         let round = (wide_as_nat h1 t + prime * (wide_as_nat h1 t % pow2 64)) / pow2 64 in
-   round % pow2 64) (pow2 64) prime;
-      mul_lemma_1 (
-  let round = (wide_as_nat h1 t + prime * (wide_as_nat h1 t % pow2 64)) / pow2 64 in
-  let round2 = (round + prime * (round % pow2 64)) / pow2 64 in
-  round2 % pow2 64) (pow2 64) prime;
-      mul_lemma_1 (
-  let round = (wide_as_nat h1 t + prime * (wide_as_nat h1 t % pow2 64)) / pow2 64 in
-  let round2 = (round + prime * (round % pow2 64)) / pow2 64 in
-  let round3 = (round2 + prime * (round2 % pow2 64)) / pow2 64 in
-  round3 % pow2 64) (pow2 64) prime;
-      assert_norm((prime * pow2 64 + (prime * pow2 64 + (prime * pow2 64 + ((pow2 64 - 1) * prime + prime * prime) / pow2 64) / pow2 64)/ pow2 64) / pow2 64 < 2 * prime);
+  Math.Lemmas.lemma_mod_mul_distr_l (wide_as_nat h2 round2) (S.modp_inv2_prime (pow2 128) S.prime) S.prime;
+  Math.Lemmas.lemma_mod_mul_distr_l (wide_as_nat h1 t * S.modp_inv2_prime (pow2 128) S.prime) (S.modp_inv2_prime (pow2 128) S.prime) S.prime;
+      SL.mul_lemma_2 (wide_as_nat h1 t % pow2 64) (pow2 64 - 1) S.prime;
+      SL.mul_lemma_ (as_nat h0 a) (as_nat h0 a) S.prime;
+      SL.mul_lemma_1 (
+         let round = (wide_as_nat h1 t + S.prime * (wide_as_nat h1 t % pow2 64)) / pow2 64 in
+   round % pow2 64) (pow2 64) S.prime;
+      SL.mul_lemma_1 (
+  let round = (wide_as_nat h1 t + S.prime * (wide_as_nat h1 t % pow2 64)) / pow2 64 in
+  let round2 = (round + S.prime * (round % pow2 64)) / pow2 64 in
+  round2 % pow2 64) (pow2 64) S.prime;
+      SL.mul_lemma_1 (
+  let round = (wide_as_nat h1 t + S.prime * (wide_as_nat h1 t % pow2 64)) / pow2 64 in
+  let round2 = (round + S.prime * (round % pow2 64)) / pow2 64 in
+  let round3 = (round2 + S.prime * (round2 % pow2 64)) / pow2 64 in
+  round3 % pow2 64) (pow2 64) S.prime;
+      assert_norm((S.prime * pow2 64 + (S.prime * pow2 64 + (S.prime * pow2 64 + ((pow2 64 - 1) * S.prime + S.prime * S.prime) / pow2 64) / pow2 64)/ pow2 64) / pow2 64 < 2 * S.prime);
   reduction_prime_2prime_8_with_carry_impl round4 result;
-  lemmaFromDomainToDomain (as_nat h0 a);
-  multiplicationInDomainNat #(fromDomain_ (as_nat h0 a)) #(fromDomain_ (as_nat h0 a))  (as_nat h0 a) (as_nat h0 a);
-  inDomain_mod_is_not_mod (fromDomain_ (as_nat h0 a) * fromDomain_ (as_nat h0 a));
+  SM.lemmaFromDomainToDomain (as_nat h0 a);
+  SM.multiplicationInDomainNat #(SM.fromDomain_ (as_nat h0 a)) #(SM.fromDomain_ (as_nat h0 a))  (as_nat h0 a) (as_nat h0 a);
+  SM.inDomain_mod_is_not_mod (SM.fromDomain_ (as_nat h0 a) * SM.fromDomain_ (as_nat h0 a));
   pop_frame()
 
 //----------------------------------------------
@@ -421,17 +415,17 @@ let fcube a result =
   fsqr a result;
   fmul result a result;
   let h1 = ST.get () in
-  lemma_mod_mul_distr_l
-    (fromDomain_ (as_nat h0 a) * fromDomain_ (as_nat h0 a))
-    (fromDomain_ (as_nat h0 a)) prime;
-  inDomain_mod_is_not_mod
-    (fromDomain_ (as_nat h0 a) * fromDomain_ (as_nat h0 a) * fromDomain_ (as_nat h0 a))
+  Math.Lemmas.lemma_mod_mul_distr_l
+    (SM.fromDomain_ (as_nat h0 a) * SM.fromDomain_ (as_nat h0 a))
+    (SM.fromDomain_ (as_nat h0 a)) S.prime;
+  SM.inDomain_mod_is_not_mod
+    (SM.fromDomain_ (as_nat h0 a) * SM.fromDomain_ (as_nat h0 a) * SM.fromDomain_ (as_nat h0 a))
 
 
 let fmul_by_2 a out =
   let h0 = ST.get () in
   fadd a a out;
-  inDomain_mod_is_not_mod (2 * fromDomain_ (as_nat h0 a))
+  SM.inDomain_mod_is_not_mod (2 * SM.fromDomain_ (as_nat h0 a))
 
 
 [@CInline]
@@ -439,11 +433,11 @@ let fmul_by_3 a result =
   let h0 = ST.get () in
   fmul_by_2 a result;
   let h1 = ST.get () in
-  assert (as_nat h1 result == toDomain_ (2 * fromDomain_ (as_nat h0 a) % prime));
+  assert (as_nat h1 result == SM.toDomain_ (2 * SM.fromDomain_ (as_nat h0 a) % S.prime));
   fadd a result result;
   let h2 = ST.get() in
-  lemma_mod_add_distr (fromDomain_ (as_nat h0 a)) (2 * fromDomain_ (as_nat h0 a)) prime;
-  inDomain_mod_is_not_mod (3 * fromDomain_ (as_nat h0 a))
+  Math.Lemmas.lemma_mod_add_distr (SM.fromDomain_ (as_nat h0 a)) (2 * SM.fromDomain_ (as_nat h0 a)) S.prime;
+  SM.inDomain_mod_is_not_mod (3 * SM.fromDomain_ (as_nat h0 a))
 
 
 [@CInline]
@@ -451,9 +445,9 @@ let fmul_by_4 a result  =
   let h0 = ST.get() in
   fmul_by_2 a result;
   fmul_by_2 result result;
-  lemma_mod_mul_distr_r 2 (2 * fromDomain_ (as_nat h0 a)) prime;
-  lemma_brackets 2 2 (fromDomain_ (as_nat h0 a));
-  inDomain_mod_is_not_mod (4 * fromDomain_ (as_nat h0 a))
+  Math.Lemmas.lemma_mod_mul_distr_r 2 (2 * SM.fromDomain_ (as_nat h0 a)) S.prime;
+  SL.lemma_brackets 2 2 (SM.fromDomain_ (as_nat h0 a));
+  SM.inDomain_mod_is_not_mod (4 * SM.fromDomain_ (as_nat h0 a))
 
 
 [@CInline]
@@ -461,6 +455,6 @@ let fmul_by_8 a result  =
   let h0 = ST.get() in
   fmul_by_4 a result;
   fmul_by_2 result result;
-  lemma_mod_mul_distr_r 2 (4 * fromDomain_ (as_nat h0 a)) prime;
-  lemma_brackets 2 4 (fromDomain_ (as_nat h0 a));
-  inDomain_mod_is_not_mod (8 * fromDomain_ (as_nat h0 a))
+  Math.Lemmas.lemma_mod_mul_distr_r 2 (4 * SM.fromDomain_ (as_nat h0 a)) S.prime;
+  SL.lemma_brackets 2 4 (SM.fromDomain_ (as_nat h0 a));
+  SM.inDomain_mod_is_not_mod (8 * SM.fromDomain_ (as_nat h0 a))
