code/ecdsap256/Hacl.Spec.P256.Math.fst
@@ -1,63 +1,22 @@
 module Hacl.Spec.P256.Math
 
-open FStar.Math.Lemmas
-open FStar.Math
 open FStar.Mul
-
 open Spec.P256
-open Hacl.Spec.P256.Lemmas
 
-#set-options "--fuel 0 --ifuel 0 --z3rlimit 200"
+#set-options "--z3rlimit 50 --fuel 0 --ifuel 0"
 
 val mod_sub: n:pos -> a:int -> b:int -> Lemma
   (requires a % n = b % n)
   (ensures  (a - b) % n = 0)
 let mod_sub n a b =
-  mod_add_both a b (-b) n
+  Math.Lemmas.mod_add_both a b (-b) n
+
 
 val sub_mod: n:pos -> a:int -> b:int -> Lemma
   (requires (a - b) % n = 0)
   (ensures  a % n = b % n)
 let sub_mod n a b =
-  mod_add_both (a - b) 0 b n
-
-val mod_same: n:pos -> Lemma (n % n = 0)
-let mod_same n = ()
-
-val euclid: n:pos -> a:int -> b:int -> r:int -> s:int -> Lemma
-  (requires (a * b) % n = 0 /\ r * n + s * a = 1)
-  (ensures  b % n = 0)
-
-let euclid n a b r s =
-  calc (==) {
-    b % n;
-    == { FStar.Math.Lemmas.distributivity_add_left (r * n) (s * a) b }
-    (r * n * b + s * a * b) % n;
-    == { FStar.Math.Lemmas.paren_mul_right s a b }
-    (r * n * b + s * (a * b)) % n;
-    == { FStar.Math.Lemmas.modulo_distributivity (r * n * b) (s * (a * b)) n }
-    ((r * n * b) % n + s * (a * b) % n) % n;
-    == { FStar.Math.Lemmas.lemma_mod_mul_distr_r s (a * b) n }
-    ((r * n * b) % n + s * ((a * b) % n) % n) % n;
-    == { assert (a * b % n = 0) }
-    ((r * n * b) % n + s * 0 % n) % n;
-    == { assert (s * 0 == 0) }
-    ((r * n * b) % n + 0 % n) % n;
-    == { FStar.Math.Lemmas.modulo_lemma 0 n }
-    ((r * n * b) % n) % n;
-    == { FStar.Math.Lemmas.lemma_mod_twice (r * n * b) n }
-    (r * n * b) % n;
-    == { FStar.Math.Lemmas.swap_mul r n; FStar.Math.Lemmas.paren_mul_right n r b }
-    (n * (r * b)) % n;
-    == { FStar.Math.Lemmas.lemma_mod_mul_distr_l n (r * b) n}
-    n % n * (r * b) % n;
-    == { mod_same n }
-    (0 * (r * b)) % n;
-    == { assert (0 * (r * b) == 0) }
-    0 % n;
-    == { FStar.Math.Lemmas.modulo_lemma 0 n }
-    0;
-  }
+  Math.Lemmas.mod_add_both (a - b) 0 b n
 
 
 val lemma_modular_multiplication_p256_2_left:
@@ -71,25 +30,23 @@ let lemma_modular_multiplication_p256_2_left a b =
   let r = 26959946654596436323893653559348051827142583427821597254581997273087 in
   let s = -26959946648319334592891477706824406424704094582978235142356758167551 in
   assert_norm (r * prime + s * pow2 256 = 1);
-  euclid prime (pow2 256) (a - b) r s;
+  FStar.Math.Euclid.euclid prime (pow2 256) (a - b) r s;
   assert ((a - b) % prime = 0);
   sub_mod prime a b;
   assert (a % prime = b % prime);
   FStar.Math.Lemmas.modulo_lemma a prime;
   FStar.Math.Lemmas.modulo_lemma b prime
 
+
+// used in Hacl.Impl.P256.Point
 val lemma_modular_multiplication_p256_2: a: nat{a < prime} -> b: nat{b < prime} ->
-  Lemma
-  (a * pow2 256 % prime = b * pow2 256 % prime <==> a == b)
+  Lemma (a * pow2 256 % prime = b * pow2 256 % prime <==> a == b)
 
 let lemma_modular_multiplication_p256_2 a b =
   Classical.move_requires_2 lemma_modular_multiplication_p256_2_left a b
 
-noextract
-let order:pos =
-  assert_norm (115792089210356248762697446949407573529996955224135760342422259061068512044369> 0);
-  115792089210356248762697446949407573529996955224135760342422259061068512044369
 
+// used in Hacl.Impl.P256.Scalar and Hacl.Impl.P256.Field
 val lemma_montgomery_mod_inverse_addition: a:nat -> Lemma (
   a * modp_inv2_prime (pow2 64) prime * modp_inv2_prime (pow2 64) prime % prime ==
   a * modp_inv2_prime (pow2 128) prime % prime)
@@ -109,6 +66,8 @@ let lemma_montgomery_mod_inverse_addition a =
     a * modp_inv2_prime (pow2 128) prime % prime;
   }
 
+
+// used in Hacl.Impl.P256.Scalar and Hacl.Impl.P256.Field
 val lemma_montgomery_mod_inverse_addition2: a:nat -> Lemma (
   a * modp_inv2_prime (pow2 128) prime * modp_inv2_prime (pow2 128) prime % prime ==
   a * modp_inv2_prime (pow2 256) prime % prime)
@@ -140,14 +99,14 @@ let lemma_montgomery_mod_inverse_addition2 a =
    r = Z(inverse_mod(2**256, order))
    r ^ (order - 1)
 *)
-val lemma_l_ferm: unit -> Lemma
-  (let r = modp_inv2_prime (pow2 256) order in
-  (pow r (order - 1) % order == 1))
+// used in Hacl.Impl.P256.Qinv
+val lemma_l_ferm: unit ->
+  Lemma (let r = modp_inv2_prime (pow2 256) order in (pow r (order - 1) % order == 1))
 
 let lemma_l_ferm () =
   let r = modp_inv2_prime (pow2 256) order in
-  assert_norm (exp (modp_inv2_prime (pow2 256) order) (order - 1)  == 1);
-  lemma_pow_mod_n_is_fpow order r (order - 1)
+  assert_norm (exp (modp_inv2_prime (pow2 256) order) (order - 1) == 1);
+  Hacl.Spec.P256.Lemmas.lemma_pow_mod_n_is_fpow order r (order - 1)
 
 
 val lemma_multiplication_not_mod_prime_left: a:nat{a < prime} -> Lemma
@@ -156,38 +115,21 @@ val lemma_multiplication_not_mod_prime_left: a:nat{a < prime} -> Lemma
 
 let lemma_multiplication_not_mod_prime_left a =
   let b = modp_inv2 (pow2 256) in
-  lemma_mod_mul_distr_r a b prime;
+  Math.Lemmas.lemma_mod_mul_distr_r a b prime;
   assert (a * b % prime == a * (b % prime) % prime);
   let r = -26959946654596436328278158470660195847911760999080590586820792680449 in
   let s = 26959946660873538059280334323183841250350249843923952699046031785985 in
   assert_norm (r * prime + s * b == 1);
-  swap_mul a b;
+  Math.Lemmas.swap_mul a b;
   assert (b * a % prime == 0);
-  euclid prime b a r s;
+  Math.Euclid.euclid prime b a r s;
   assert (a % prime == 0);
-  small_mod a prime
+  Math.Lemmas.small_mod a prime
 
+
+// used in Hacl.Impl.P256.PointAdd, Hacl.Impl.P256.PointMul, Hacl.Impl.P256.Point
 val lemma_multiplication_not_mod_prime: a:nat{a < prime} ->
   Lemma (a * (modp_inv2 (pow2 256)) % prime == 0 <==> a == 0)
 
 let lemma_multiplication_not_mod_prime a =
   Classical.move_requires lemma_multiplication_not_mod_prime_left a
-
-
-val lemma_modular_multiplication_p256: a:nat{a < prime} -> b:nat{b < prime} -> Lemma
-  (requires a * modp_inv2 (pow2 256) % prime == b * modp_inv2 (pow2 256) % prime)
-  (ensures  a == b)
-
-let lemma_modular_multiplication_p256 a b =
-  let c = modp_inv2 (pow2 256) in
-  mod_sub prime (a * c) (b * c);
-  assert (c * (a - b) % prime = 0);
-  let r = -26959946654596436328278158470660195847911760999080590586820792680449 in
-  let s = 26959946660873538059280334323183841250350249843923952699046031785985 in
-  assert_norm (r * prime + s * c = 1);
-  euclid prime c (a - b) r s;
-  assert ((a - b) % prime = 0);
-  sub_mod prime a b;
-  assert (a % prime == b % prime);
-  FStar.Math.Lemmas.modulo_lemma a prime;
-  FStar.Math.Lemmas.modulo_lemma b prime
