code/ecdsap256/Hacl.Impl.P256.Field.fsti
@@ -8,17 +8,18 @@ module ST = FStar.HyperStack.ST
 open Lib.IntTypes
 open Lib.Buffer
 
-open Spec.P256
-open Hacl.Spec.P256.MontgomeryMultiplication
 open Hacl.Spec.P256.Felem
 
-#set-options "--z3rlimit 50"
+module S = Spec.P256
+module SM = Hacl.Spec.P256.MontgomeryMultiplication
+
+#set-options "--z3rlimit 50 --fuel 0 --ifuel 0"
 
 val fmod_short: x:felem -> res:felem -> Stack unit
   (requires fun h ->
     live h x /\ live h res /\ eq_or_disjoint x res)
   (ensures fun h0 _ h1 -> modifies (loc res) h0 h1 /\
-    as_nat h1 res == as_nat h0 x % prime)
+    as_nat h1 res == as_nat h0 x % S.prime)
 
 
 // NOTE: changed precondition `eq_or_disjoint x y`
@@ -26,21 +27,21 @@ val fadd: x:felem -> y:felem -> res:felem -> Stack unit
   (requires fun h0 ->
     live h0 x /\ live h0 y /\ live h0 res /\
     eq_or_disjoint x y /\ eq_or_disjoint x res /\ eq_or_disjoint y res /\
-    as_nat h0 x < prime /\ as_nat h0 y < prime)
+    as_nat h0 x < S.prime /\ as_nat h0 y < S.prime)
   (ensures  fun h0 _ h1 -> modifies (loc res) h0 h1 /\
-    as_nat h1 res == (as_nat h0 x + as_nat h0 y) % prime /\
-    as_nat h1 res == toDomain_ ((fromDomain_ (as_nat h0 x) + fromDomain_ (as_nat h0 y)) % prime))
+    as_nat h1 res == (as_nat h0 x + as_nat h0 y) % S.prime /\
+    as_nat h1 res == SM.toDomain_ ((SM.fromDomain_ (as_nat h0 x) + SM.fromDomain_ (as_nat h0 y)) % S.prime))
 
 
 inline_for_extraction noextract
 val fdouble: x:felem -> res:felem -> Stack unit
   (requires fun h0 ->
     live h0 x /\ live h0 res /\ eq_or_disjoint x res /\
-    as_nat h0 x < prime)
+    as_nat h0 x < S.prime)
   (ensures fun h0 _ h1 -> modifies (loc res) h0 h1 /\
-    as_nat h1 res == (2 * as_nat h0 x) % prime /\
-    as_nat h1 res < prime /\
-    as_nat h1 res == toDomain_ (2 * fromDomain_ (as_nat h0 x) % prime))
+    as_nat h1 res == (2 * as_nat h0 x) % S.prime /\
+    as_nat h1 res < S.prime /\
+    as_nat h1 res == SM.toDomain_ (2 * SM.fromDomain_ (as_nat h0 x) % S.prime))
 
 
 // NOTE: changed precondition `eq_or_disjoint x y`
@@ -48,41 +49,41 @@ val fsub: x:felem -> y:felem -> res:felem -> Stack unit
   (requires fun h0 ->
     live h0 res /\ live h0 x /\ live h0 y /\
     eq_or_disjoint x y /\ eq_or_disjoint x res /\ eq_or_disjoint y res /\
-    as_nat h0 x < prime /\ as_nat h0 y < prime)
+    as_nat h0 x < S.prime /\ as_nat h0 y < S.prime)
   (ensures fun h0 _ h1 -> modifies (loc res) h0 h1 /\
-    as_nat h1 res == (as_nat h0 x - as_nat h0 y) % prime /\
-    as_nat h1 res == toDomain_ ((fromDomain_ (as_nat h0 x) - fromDomain_ (as_nat h0 y)) % prime))
+    as_nat h1 res == (as_nat h0 x - as_nat h0 y) % S.prime /\
+    as_nat h1 res == SM.toDomain_ ((SM.fromDomain_ (as_nat h0 x) - SM.fromDomain_ (as_nat h0 y)) % S.prime))
 
 
 // TODO: rename
 val montgomery_multiplication_buffer_by_one: a:felem -> res:felem -> Stack unit
   (requires fun h ->
-    live h a /\ live h res /\ as_nat h a < prime)
+    live h a /\ live h res /\ as_nat h a < S.prime)
   (ensures  fun h0 _ h1 -> modifies (loc res) h0 h1 /\
-    as_nat h1 res = (as_nat h0 a * modp_inv2_prime (pow2 256) prime) % prime /\
-    as_nat h1 res = fromDomain_ (as_nat h0 a))
+    as_nat h1 res = (as_nat h0 a * SM.mont_R_inv) % S.prime /\
+    as_nat h1 res = SM.fromDomain_ (as_nat h0 a))
 
 
 val fmul: a:felem -> b:felem -> res:felem -> Stack unit
   (requires fun h ->
     live h a /\ live h b /\ live h res /\
     eq_or_disjoint a b /\
-    as_nat h a < prime /\ as_nat h b < prime)
+    as_nat h a < S.prime /\ as_nat h b < S.prime)
   (ensures fun h0 _ h1 -> modifies (loc res) h0 h1 /\
-    as_nat h1 res < prime /\
-    as_nat h1 res = (as_nat h0 a * as_nat h0 b * modp_inv2_prime (pow2 256) prime) % prime /\
-    as_nat h1 res = toDomain_ (fromDomain_ (as_nat h0 a) * fromDomain_ (as_nat h0 b) % prime) /\
-    as_nat h1 res = toDomain_ (fromDomain_ (as_nat h0 a) * fromDomain_ (as_nat h0 b)))
+    as_nat h1 res < S.prime /\
+    as_nat h1 res = (as_nat h0 a * as_nat h0 b * SM.mont_R_inv) % S.prime /\
+    as_nat h1 res = SM.toDomain_ (SM.fromDomain_ (as_nat h0 a) * SM.fromDomain_ (as_nat h0 b) % S.prime) /\
+    as_nat h1 res = SM.toDomain_ (SM.fromDomain_ (as_nat h0 a) * SM.fromDomain_ (as_nat h0 b)))
 
 
 val fsqr: a:felem -> res:felem -> Stack unit
   (requires fun h ->
-    live h a /\ live h res /\ as_nat h a < prime)
+    live h a /\ live h res /\ as_nat h a < S.prime)
   (ensures  fun h0 _ h1 -> modifies (loc res) h0 h1 /\
-    as_nat h1 res < prime /\
-    as_nat h1 res = (as_nat h0 a * as_nat h0 a * modp_inv2_prime (pow2 256) prime) % prime /\
-    as_nat h1 res = toDomain_ (fromDomain_ (as_nat h0 a) * fromDomain_ (as_nat h0 a) % prime) /\
-    as_nat h1 res = toDomain_ (fromDomain_ (as_nat h0 a) * fromDomain_ (as_nat h0 a)))
+    as_nat h1 res < S.prime /\
+    as_nat h1 res = (as_nat h0 a * as_nat h0 a * SM.mont_R_inv) % S.prime /\
+    as_nat h1 res = SM.toDomain_ (SM.fromDomain_ (as_nat h0 a) * SM.fromDomain_ (as_nat h0 a) % S.prime) /\
+    as_nat h1 res = SM.toDomain_ (SM.fromDomain_ (as_nat h0 a) * SM.fromDomain_ (as_nat h0 a)))
 
 
 ///  Special cases of the above functions
@@ -90,49 +91,49 @@ val fsqr: a:felem -> res:felem -> Stack unit
 val fcube: a:felem -> res:felem -> Stack unit
   (requires fun h ->
     live h a /\ live h res /\ disjoint a res /\
-    as_nat h a < prime)
+    as_nat h a < S.prime)
   (ensures fun h0 _ h1 -> modifies (loc res) h0 h1 /\
-    as_nat h1 res < prime /\
-    as_nat h1 res = toDomain_ (fromDomain_ (as_nat h0 a) * fromDomain_ (as_nat h0 a) * fromDomain_ (as_nat h0 a) % prime) /\
-    as_nat h1 res = toDomain_ (fromDomain_ (as_nat h0 a) * fromDomain_ (as_nat h0 a) * fromDomain_ (as_nat h0 a)))
+    as_nat h1 res < S.prime /\
+    as_nat h1 res = SM.toDomain_ (SM.fromDomain_ (as_nat h0 a) * SM.fromDomain_ (as_nat h0 a) * SM.fromDomain_ (as_nat h0 a) % S.prime) /\
+    as_nat h1 res = SM.toDomain_ (SM.fromDomain_ (as_nat h0 a) * SM.fromDomain_ (as_nat h0 a) * SM.fromDomain_ (as_nat h0 a)))
 
 
 inline_for_extraction noextract
 val fmul_by_2: a:felem -> res:felem -> Stack unit
   (requires fun h ->
     live h a /\ live h res /\ eq_or_disjoint a res /\
-    as_nat h a < prime)
+    as_nat h a < S.prime)
   (ensures fun h0 _ h1 -> modifies (loc res) h0 h1 /\
-    as_nat h1 res == toDomain_ (2 * fromDomain_ (as_nat h0 a) % prime) /\
-    as_nat h1 res == toDomain_ (2 * fromDomain_ (as_nat h0 a)) /\
-    as_nat h1 res < prime)
+    as_nat h1 res == SM.toDomain_ (2 * SM.fromDomain_ (as_nat h0 a) % S.prime) /\
+    as_nat h1 res == SM.toDomain_ (2 * SM.fromDomain_ (as_nat h0 a)) /\
+    as_nat h1 res < S.prime)
 
 
 val fmul_by_3: a:felem -> res:felem -> Stack unit
   (requires fun h ->
     live h a /\ live h res /\ disjoint a res /\
-    as_nat h a < prime)
+    as_nat h a < S.prime)
   (ensures fun h0 _ h1 -> modifies (loc res) h0 h1 /\
-    as_nat h1 res < prime /\
-    as_nat h1 res == toDomain_ (3 * fromDomain_ (as_nat h0 a) % prime) /\
-    as_nat h1 res == toDomain_ (3 * fromDomain_ (as_nat h0 a)))
+    as_nat h1 res < S.prime /\
+    as_nat h1 res == SM.toDomain_ (3 * SM.fromDomain_ (as_nat h0 a) % S.prime) /\
+    as_nat h1 res == SM.toDomain_ (3 * SM.fromDomain_ (as_nat h0 a)))
 
 
 val fmul_by_4: a:felem -> res:felem -> Stack unit
   (requires fun h ->
     live h a /\ live h res /\ eq_or_disjoint a res /\
-    as_nat h a < prime)
+    as_nat h a < S.prime)
   (ensures fun h0 _ h1 -> modifies (loc res) h0 h1 /\
-    as_nat h1 res < prime /\
-    as_nat h1 res == toDomain_ (4 * fromDomain_ (as_nat h0 a) % prime) /\
-    as_nat h1 res == toDomain_ (4 * fromDomain_ (as_nat h0 a)))
+    as_nat h1 res < S.prime /\
+    as_nat h1 res == SM.toDomain_ (4 * SM.fromDomain_ (as_nat h0 a) % S.prime) /\
+    as_nat h1 res == SM.toDomain_ (4 * SM.fromDomain_ (as_nat h0 a)))
 
 
 val fmul_by_8: a:felem -> res:felem -> Stack unit
   (requires fun h ->
     live h a /\ live h res /\ disjoint a res /\
-    as_nat h a < prime)
+    as_nat h a < S.prime)
   (ensures fun h0 _ h1 -> modifies (loc res) h0 h1 /\
-    as_nat h1 res < prime /\
-    as_nat h1 res == toDomain_ (8 * fromDomain_ (as_nat h0 a) % prime) /\
-    as_nat h1 res == toDomain_ (8 * fromDomain_ (as_nat h0 a)))
+    as_nat h1 res < S.prime /\
+    as_nat h1 res == SM.toDomain_ (8 * SM.fromDomain_ (as_nat h0 a) % S.prime) /\
+    as_nat h1 res == SM.toDomain_ (8 * SM.fromDomain_ (as_nat h0 a)))
